src/examples/Kuiper.ArrayView.Test.EvenOdds.fst
@@ -109,6 +109,7 @@ fn foo_odd (a : varray (odd_view u32 100))
   varray_read #_ #_ #_ #(_cview_odd #_ _ solve) a 10sz;
 }
 
+#push-options "--z3rlimit 30"
 fn test (a : gpu_array u32 100)
   (#v0 : erased (lseq u32 100))
   preserves gpu
@@ -143,3 +144,4 @@ fn test (a : gpu_array u32 100)
 
   res
 }
+#pop-options
