src/lib/kuiper/Kuiper.GhostPull.fsti
@@ -1,0 +1,4 @@
+module Kuiper.GhostPull
+
+(* An axiom. Used to be in the F* library. *)
+val ghost_pull (#a #b:Type) (f: a -> GTot b) : GTot (g:(a -> b) { forall x. f x == g x })
