verify.mk
@@ -114,6 +114,7 @@ FSTAR_FLAGS += --ext optimize_let_vc
 FSTAR_FLAGS += --ext __unrefine
 FSTAR_FLAGS += --ext context_pruning
 FSTAR_FLAGS += --ext no_krml_private
+FSTAR_FLAGS += --warn_error -288 # using has_type (we only use it in SMT patterns)
 # FSTAR_FLAGS += --ext krml_inline_all
 # FSTAR_FLAGS += --error_contexts true
 FSTAR_FLAGS += $(OTHERFLAGS)
